TODO.md
@@ -13,9 +13,9 @@
 * Rename `osirisGS_gen` to something less ugly.
 * In `steps.v`, we could use `nsteps` from `stdpp`.
 
-* `dconcatenating` is not built on the same model as `concatenating`
+* `ret_dconcat` is not built on the same model as `concatenating`
   and does not appear at the root (it appear under `bind`). Fix?
-* `concatenating`, `dconcatenating` and other hacks
+* `concatenating`, `ret_dconcat` and other hacks
   should appear in `evalprime`, not `eval`.
 
 ## Iris machinery
